cleanup

src/theory/bir/bir_promising_diamondScript.sml
@@ -1,18 +1,15 @@
-open HolKernel Parse;
+open HolKernel Parse boolLib bossLib;
 open bir_promisingTheory;
 open bir_programTheory;
+open bir_valuesTheory;
+open bir_expTheory;
 open finite_mapTheory;
 
 val _ = new_theory "bir_promising_diamond";
 
-Definition bir_promising_sim_rel_def:
-  sim_rel (cores:num |-> core_t,M:mem_msg_t list) (cores',M') =
-   (cores = cores' /\ M = M')
-End
-
 Definition bir_promise_step_def:
   promise_step cid (cores,M) (cores',M') =
-     (parstep cid cores M cores' M' /\ ~(M = M'))
+  (parstep cid cores M cores' M' /\ ~(M = M'))
 End
 
 Definition bir_nonpromise_step_def:
@@ -20,50 +17,507 @@ Definition bir_nonpromise_step_def:
   (parstep cid cores M cores' M' /\ (M = M'))
 End
 
+Definition latest_def:
+  latest l 0 M = 0
+  /\ latest l (SUC t) M =
+  case oEL t M of
+    SOME msg =>
+      if l = msg.loc then SUC t else latest l t M
+  | _ => latest l t M
+End
+
+Definition well_formed_fwdb_def:
+ well_formed_fwdb l M coh_t fwd =
+   (fwd.fwdb_time <= latest l coh_t M
+    /\ fwd.fwdb_view <= fwd.fwdb_time
+    /\ ?v. mem_read M l fwd.fwdb_time = SOME v)
+End
+(*
+Definition well_formed_xclb_def:
+  well_formed_xclb M coh_t xclb =
+  (xclb.xclb_time <= latest xclb.xclb_loc coh_t M
+   /\ xclb.xclb_view <= coh_t
+   /\ ?v. mem_read M xclb.xclb_loc xclb.xclb_time = SOME v)
+End
+*)
+
+Definition well_formed_viewenv_def:
+  well_formed_viewenv viewenv M =
+  !var v. FLOOKUP viewenv var = SOME v
+  ==>
+  v <= LENGTH M
+End
+
+Definition well_formed_def:
+  well_formed cid M s =
+  ( well_formed_viewenv s.bst_viewenv M
+    /\ (!l. s.bst_coh(l) <= LENGTH M)
+     /\ s.bst_v_rNew <= LENGTH M
+     /\ s.bst_v_rOld <= LENGTH M
+     /\ s.bst_v_wNew <= LENGTH M
+     /\ s.bst_v_wOld <= LENGTH M
+     /\ s.bst_v_CAP <= LENGTH M
+     /\ s.bst_v_Rel <= LENGTH M
+     /\ (!l. well_formed_fwdb l M (s.bst_coh(l)) (s.bst_fwdb(l)))
+(*     /\ (!xclb. s.bst_xclb = SOME xclb ==> well_formed_xclb M (s.bst_coh(xclb.loc) xclb)) *)
+     /\ (!t. MEM t s.bst_prom ==> t <= LENGTH M)
+     /\ (!t msg.
+           (oEL t M = SOME msg
+            /\ msg.cid = cid
+            /\ s.bst_coh(msg.loc) < t)
+           ==>
+           MEM t s.bst_prom)
+    )
+End
+
+Triviality mem_get_SOME:
+  !l t M msg.
+    mem_get M l t = SOME msg
+    ==>
+    l = msg.loc
+Proof
+  Cases_on ‘t’
+  >> fs[mem_get_def, mem_default_def]
+  >> rpt strip_tac
+  >> Cases_on ‘oEL n M’
+  >> gvs[]
+QED
+
+Theorem mem_get_mem_read:
+  !M l t v.
+    mem_read M l t = SOME v
+    ==>
+    ?m. mem_get M l t = SOME m /\ m.val = v
+Proof
+  Induct_on ‘t’ >- fs[mem_read_def, mem_get_def]
+  >> rpt strip_tac
+  >> fs[mem_read_def, mem_get_def]
+  >> Cases_on ‘oEL t M’
+  >- fs[]
+  >> Cases_on ‘x.loc = l’ >- fs[]
+  >> fs[]
+QED
+
+Theorem mem_get_append:
+  !t M l msg.
+    t <= LENGTH M ==> mem_get (M++[msg]) l t = mem_get M l t
+Proof
+  rpt strip_tac
+  >> Cases_on ‘t’
+  >> fs[mem_get_def] (* discharges 0 case, SUC remains *)
+  >> fs[listTheory.oEL_THM, rich_listTheory.EL_APPEND1]
+QED
+
 Triviality mem_read_some:
   !M l t v.
     mem_read M l t = SOME v ==> t <= LENGTH M \/ (t = 0 /\ v = mem_default_value)
 Proof
   Induct_on ‘t’
   >> rpt strip_tac
-  >> fs[mem_read_def]
+  >> fs[mem_read_def,mem_get_def]
   >> Cases_on ‘oEL t M’
-  >> fs[mem_read_aux_def,listTheory.oEL_EQ_EL, listTheory.oEL_def]
+  >> fs[listTheory.oEL_EQ_EL, listTheory.oEL_def]
 QED
 
+Theorem programs_unchanged:
+  !cid T1 T2 M1 M2.
+    parstep cid T1 M1 T2 M2 ==>
+    !p s p' s'.
+      FLOOKUP T1 cid = SOME (Core cid p s)
+      /\ FLOOKUP T2 cid = SOME (Core cid p' s')
+      ==> p = p'
+Proof
+  rpt strip_tac
+  >> fs[parstep_cases]
+  >> last_assum (fn th => fs [th,FLOOKUP_UPDATE])
+QED
 
+Triviality latest_bound:
+!l t M.
+  latest l t M <= t
+Proof
+  Induct_on ‘t’ >> fs[latest_def]
+  >> rpt strip_tac
+  >> ‘latest l t M <= t’ by fs[]
+  >> Cases_on ‘oEL t M’
+  >> Cases_on ‘l = x.loc’
+  >> fs[]
+QED
+
+Triviality latest_exact:
+!l t M msg.
+  mem_get M l t = SOME msg
+  ==>
+  latest l t M = t
+Proof
+  Cases_on ‘t’
+  >> rpt strip_tac
+  >> fs[latest_def]
+  >> Cases_on ‘oEL n M’
+  >- fs[mem_get_def]
+  >> ‘x = msg’ by fs[mem_get_def]
+  >> ‘l = msg.loc’ by (drule mem_get_SOME >> fs[])
+  >> gvs[]
+QED
+
+Triviality latest_sound:
+  !l t M. ?msg.
+            mem_get M l (latest l t M) = SOME msg
+            /\ msg.loc = l
+Proof
+  Induct_on ‘t’ >- fs[latest_def, mem_get_def, mem_default_def]
+  >> rpt strip_tac
+  >> fs[latest_def]
+  >> Cases_on ‘oEL t M’
+  >> fs[]
+  >> Cases_on ‘l = x.loc’ >- fs[mem_get_def]
+  >> fs[]
+QED
+
+Theorem latest_is_latest:
+  !l t M t' msg.
+    latest l t M <= t' /\ t' <= t
+    /\ mem_get M l t' = SOME msg
+    ==>
+    t' = latest l t M
+Proof
+  Induct_on ‘t’ >- fs[latest_def]
+  >> rpt strip_tac
+  >> qspecl_then [‘l’, ‘SUC t’, ‘M’] assume_tac latest_sound
+  >> Cases_on ‘t' = SUC t’ >- fs[latest_exact]
+  >> ‘t' <= t’ by decide_tac
+  >> fs[latest_def]
+  >> Cases_on ‘oEL t M’
+  >> Cases_on ‘l = x.loc’
+  >> fs[]
+QED
+
+Theorem latest_monotonicity:
+!l M t1 t2.
+  t1 <= t2 ==> latest l t1 M <= latest l t2 M
+Proof
+  rpt strip_tac
+  >> ‘?msg.mem_get M l (latest l t2 M) = SOME msg /\ msg.loc = l’
+    by fs[latest_sound]
+  >> ‘latest l t1 M <= t1’ by fs[latest_bound]
+  >> ‘latest l t2 M <= t2’ by fs[latest_bound]
+  >> Cases_on ‘t1 <= latest l t2 M’
+  >| [fs[]
+      ,
+      ‘latest l t2 M < t1’ by decide_tac
+      >> ‘?msg.mem_get M l (latest l t1 M) = SOME msg /\ msg.loc = l’
+        by fs[latest_sound]
+      >> spose_not_then assume_tac
+      >> ‘latest l t2 M <= latest l t1 M’ by decide_tac
+      >> ‘latest l t1 M <= t2’ by decide_tac
+      >> ‘latest l t1 M = latest l t2 M’
+         by (irule latest_is_latest >> fs[])
+      >> fs[]]
+QED
+
+Theorem latest_spec:
+  !l t M l1.
+    (l1 = latest l t M)
+    ==>
+    (?msg.
+      mem_get M l l1 = SOME msg
+      /\ msg.loc = l
+      /\
+      !t'. l1 < t' /\ t' <= t
+           ==>
+           mem_get M l t' = NONE)
+Proof
+  rpt strip_tac
+  >> qspecl_then [‘l’, ‘t’, ‘M’] assume_tac latest_sound
+  >> fs[]
+  >> rpt strip_tac
+  >> spose_not_then assume_tac
+  >> Cases_on ‘mem_get M l t'’ >- fs[]
+  >> ‘latest l t' M = t'’ by fs[latest_exact]
+  >> ‘latest l t' M <= latest l t M’ by fs[latest_monotonicity]
+  >> rw[]
+QED
+
+Theorem latest_idempotency:
+  !l t M.
+    latest l (latest l t M) M = latest l t M
+Proof
+  rpt strip_tac
+  >> ‘?msg. mem_get M l (latest l t M) = SOME msg /\ msg.loc = l’
+    by fs[latest_sound]
+  >> fs[latest_exact]
+QED
+
+Theorem latest_max:
+!l M t1 t2.
+   latest l t1 M <= latest l (MAX t1 t2) M
+   /\ latest l t2 M <= latest l (MAX t1 t2) M
+Proof
+  fs[latest_monotonicity]
+QED
+
+Theorem clstep_preserves_wf_fwdb:
+!p cid s M prom s'.
+(!l. well_formed_fwdb l M (s.bst_coh l) (s.bst_fwdb l))
+/\ clstep p cid s M prom s'
+==>
+(!l. well_formed_fwdb l M (s'.bst_coh l) (s'.bst_fwdb l))
+Proof
+rpt strip_tac
+>> fs[clstep_cases]
+>> fs[well_formed_fwdb_def, latest_def]
+>|
+[ (* read *)
+Cases_on ‘l = l'’
+>| [
+‘(s.bst_fwdb l').fwdb_time ≤ latest l' (s.bst_coh l') M’ by fs[]
+>> suff_tac “latest l' (s.bst_coh l') M <=
+             latest l'
+                    (MAX (s.bst_coh l')
+                     (MAX
+                      (MAX
+                       (MAX (MAX v_addr s.bst_v_rNew)
+                        (if acq ∧ rel then s.bst_v_Rel else 0))
+                       (if acq ∧ rel then MAX s.bst_v_rOld s.bst_v_wOld else 0))
+                      (mem_read_view (s.bst_fwdb l') t))) M” >- fs[]
+>> fs[latest_max]
+,
+fs[]
+],
+  (* write *)
+  Cases_on ‘l = l'’
+  >| [
+    ‘mem_read M l' v_post = SOME v’ by fs[mem_read_def]
+    >> fs[]
+    >> ‘v_post = latest l' v_post M’ by fs[latest_exact]
+    >> ‘latest l' v_post M <= latest l' (MAX (s.bst_coh l') v_post) M’ suffices_by fs[]
+    >> fs[latest_max]
+    , fs[]
+  ]
+  , (* amo *)
+  Cases_on ‘l = l'’
+  >| [
+      EVAL_TAC
+      >> ‘mem_read M l t_w = SOME v_w’ by fs[mem_read_def]
+      >> fs[]
+      >> ‘t_w = latest l t_w M’  by fs[latest_exact]
+      >> ‘latest l' t_w M <= latest l' (MAX (s.bst_coh l') t_w) M’
+         suffices_by gvs[]
+      >> fs[latest_max]
+      ,
+      EVAL_TAC
+      >> fs[]
+      >> ‘?v.mem_read M l (s.bst_fwdb l).fwdb_time = SOME v’ by fs[]
+      >> qexists_tac ‘v’
+      >> ‘?m. mem_get M l (s.bst_fwdb l).fwdb_time = SOME m /\ m.val = v’ by fs[mem_get_mem_read]
+      >> fs[]
+    ]
+  ,
+  (* branch *)
+  drule bir_exec_stmt_mc_invar >> strip_tac >> fs[]
+  ,
+  (* generic *)
+  drule bir_exec_stmt_mc_invar >> strip_tac >> fs[]
+]
+QED
+
+Theorem bir_eval_view_of_exp_wf:
+!a_e env viewenv M v_addr.
+ well_formed_viewenv viewenv M
+ /\ v_addr = bir_eval_view_of_exp a_e viewenv
+ ==>
+ v_addr <= LENGTH M
+Proof
+  fs[well_formed_viewenv_def]
+  >> Induct_on ‘a_e’
+  >> fs[bir_eval_view_of_exp_def]
+  >> rpt strip_tac
+  >- (Cases_on ‘FLOOKUP viewenv b’ >- fs[]
+      >> first_assum drule >> fs[])
+  >> first_assum drule
+  >> last_assum drule >> fs[]
+QED
+
+Triviality mem_read_view_wf_fwdb:
+!l M coh_t fwd t.
+well_formed_fwdb l M coh_t fwd
+/\ t <= LENGTH M
+==>
+mem_read_view fwd t ≤ LENGTH M
+Proof
+  rpt strip_tac
+  >> fs[mem_read_view_def, well_formed_fwdb_def]
+  >> CASE_TAC
+  >> gvs[]
+QED
+
+Theorem clstep_preserves_wf:
+!p cid s M prom s'.
+  well_formed cid M s
+  /\ clstep p cid s M prom s'
+==>
+  well_formed cid M s'
+Proof
+  cheat
+QED
+(* Incomplete proof for time reasons,
+   but it should be straightforward
+
+  rpt strip_tac
+  >> fs[well_formed_def]
+  >> drule_then imp_res_tac clstep_preserves_wf_fwdb
+  >> fs[clstep_cases]
+    >|
+  [ (* read *)
+    ‘v_addr <= LENGTH M’
+     by (fs[bir_eval_exp_view_def]
+         >> drule bir_eval_view_of_exp_wf
+         >> fs[])
+    >> fs[well_formed_viewenv_def]
+    >> Cases_on ‘acq /\ rel’
+    >|
+    [
+      irule_at Any mem_read_view_wf_fwdb
+      >> qexists_tac ‘l’ >> qexists_tac ‘s.bst_coh l’
+      >> gvs[]
+      >> conj_asm1_tac
+      >-
+        (‘t <= LENGTH M \/ (t = 0 /\ v = mem_default_value)’
+         by metis_tac[mem_read_some]
+         >> fs[])
+      >> rw[]
+      >> Cases_on ‘var' = var’
+      >> gvs[FLOOKUP_DEF, FLOOKUP_UPDATE]
+      >> irule mem_read_view_wf_fwdb
+      >> fs[]
+      >> qexists_tac ‘s.bst_coh l’ >> qexists_tac ‘l’
+      >> fs[]
+      ,
+      cheat
+    ]
+  , proof follows here
+  ]
+*)
+
+Definition valid_index_def:
+valid_index i rho =
+(i >= 0 /\ i < LENGTH rho)
+End
+
+Definition low_eq_view_def:
+low_eq_view (N:num) v1 v2 =
+  if v1 <= N /\ v2 <= N then v1 = v2 else T
+End
+
+Definition low_eq_fwd_def:
+low_eq_fwd (N:num) fwd1 fwd2 =
+  low_eq_view N fwd1.fwdb_view fwd2.fwdb_view
+End
+
+Definition low_eq_xclb_def:
+low_eq_xclb N (SOME xcl1) (SOME xcl2) =
+  low_eq_view N xcl1.xclb_view xcl2.xclb_view
+/\ low_eq_xclb N _ _ = T
+End
+
+Definition low_eq_def:
+low_eq (N:num) s s' =
+(low_eq_view N s.bst_v_rOld s'.bst_v_rOld
+ /\ low_eq_view N s.bst_v_wOld s'.bst_v_wOld
+ /\ low_eq_view N s.bst_v_rNew s'.bst_v_rNew
+ /\ low_eq_view N s.bst_v_wNew s'.bst_v_wNew
+ /\ low_eq_view N s.bst_v_CAP s'.bst_v_CAP
+ /\ low_eq_view N s.bst_v_Rel s'.bst_v_Rel
+ /\ (!var v1 v2.
+       FLOOKUP s.bst_viewenv var = SOME v1
+       /\ FLOOKUP s'.bst_viewenv var = SOME v2
+       ==> low_eq_view N v1 v2)
+ /\ (!l. low_eq_view N (s.bst_coh l) (s'.bst_coh l))
+ /\ (!l. low_eq_fwd N (s.bst_fwdb l) (s'.bst_fwdb l))
+ /\ low_eq_xclb N s.bst_xclb s'.bst_xclb
+)
+End
+
+(* Monotonicity of vCAP *)
+
+(* Monotonicity of fence? *)
+
+(*Unwinding conditions
+
+NI-like lemma:
+cstep_seq_time p cid t s M s1 M'
+/\ low_eq k s s'
+==>
+?s2 t'.
+cstep_seq_time p cid t' s' M s2 M'
+/\ low-eq k s1 s2
+*)
+
+Definition is_read_stmt_def:
+  is_read_stmt p s l t v_pre =
+  ?M var a_e opt_cast xcl acq rel v_addr v.
+    bir_get_stmt p s.bst_pc =
+    BirStmt_Read var a_e opt_cast xcl acq rel
+    /\ (SOME l, v_addr) = bir_eval_exp_view a_e s.bst_environ s.bst_viewenv
+    /\ mem_read M l t = SOME v
+    /\ v_pre = MAX (MAX (MAX v_addr s.bst_v_rNew) (if (acq /\ rel) then s.bst_v_Rel else 0))
+                   (if (acq /\ rel) then (MAX s.bst_v_rOld s.bst_v_wOld) else 0)
+End
+
+(* Some attempts at formulating
+   the NI-like properties:
+
+Theorem unwinding_cstep_seq:
+!p cid t s M s1 M' k.
+  cstep_seq_time p cid t s M s1 M'
+  /\ low_eq k s s'
+  ==>
+  ?s2 t'.
+    (cstep_seq_time p cid t' s' M s2 M'
+     /\ low-eq k s1 s2)
+Proof
+  cheat
+QED
+
+Theorem cert_future_irrelevance:
+!p cid s M rho i j.
+rho IN certifying_traces p cid s M
+valid_index i rho /\ valid_index j rho
+/\ time = timestamp_at i rho
+/\ is_mem_op i rho
+/\ timestamp_at j rho > time
+==>
+!rho'.
+similar_trace rho rho' (* ?? *)
+/\ ~(timestamp_at j rho' = timestamp_at j rho)
+/\ timestamp_at j rho' = LENGTH M + 1 (* ?? *)
+==>
+rho' IN certifying_traces p cid s (M++[promise]) (* ?? *)
+Proof
+  cheat
+QED
+*)
+
+Triviality mem_read_append:
+!t M l msg.
+     t <= LENGTH M ==> mem_read (M++[msg]) l t = mem_read M l t
+Proof
+  fs[mem_read_def,mem_get_append]
+QED
+
+(* More general version, but not needed so far
 Triviality mem_read_append2:
   !t M l M'.
     t <= LENGTH M ==> mem_read (M++M') l t = mem_read M l t
 Proof
   rewrite_tac [GSYM listTheory.SNOC_APPEND]
-  >> Induct_on ‘t’ 
+  >> Induct_on ‘t’
   >> fs[mem_read_def]
   >> rpt strip_tac
-  >> ‘t <= LENGTH M’ by decide_tac
-  >> LAST_ASSUM drule >> rw[mem_read_def, mem_read_aux_def]
+  >> rw[mem_read_def, mem_get_def]
   >> fs[listTheory.oEL_THM, listTheory.EL_SNOC, listTheory.EL_APPEND_EQN]
 QED
-
-  
-Triviality mem_read_append:
-!t M l msg.
-     t <= LENGTH M ==> mem_read (M++[msg]) l t = mem_read M l t
-Proof
-  rewrite_tac [GSYM listTheory.SNOC_APPEND]
-  >> Induct_on ‘t’ 
-  >> fs[mem_read_def]
-  >> rpt strip_tac
-  >> ‘t <= LENGTH M’ by decide_tac
-  >> LAST_ASSUM drule >> rw[mem_read_def, mem_read_aux_def]
-  >> fs[listTheory.oEL_THM, listTheory.EL_SNOC]
-QED
-
-Triviality sim_rel_eq:
-  sim_rel (cores,M) (cores',M') = (cores = cores' /\ M = M')
-Proof
-  fs[bir_promising_sim_rel_def]
-QED
+*)
 
 Theorem promise_inversion:
 !cid cores M cores' M'.
@@ -223,7 +677,7 @@ Proof
     >> Cases_on ‘MEM x (bir_labels_of_program p)’
     >> fs[]
 QED
-  
+
 Theorem bir_exec_stmtE_promise_commutes:
 !p b s f.
  bir_exec_stmtE p b (s with bst_prom updated_by f) = bir_exec_stmtE p b s with bst_prom updated_by f
@@ -295,13 +749,13 @@ Induct_on ‘clstep’
   [drule mem_read_some >> strip_tac >> fs[mem_read_append]
   ,fs[]
   , (* quantifier case *)
-  fs[]
-  >> qpat_assum ‘!t''._’ (fn th => drule (Q.SPEC ‘t'’ th))
+  qpat_assum ‘!t''._’ (fn th => drule (Q.SPEC ‘t'’ th))
   >> rpt strip_tac
-  >> ‘t' ≤ MAX v_pre (s.bst_coh l)’ by fs[bir_state_t_accfupds]
-  >> ‘∃msg. oEL (t'-1) M1 = SOME msg ∧ msg.loc ≠ l’ by fs[]
-  >> Q.EXISTS_TAC ‘msg''’
+  >> ‘¬mem_is_loc M1 t' l’ by fs[]
   >> fs[listTheory.oEL_EQ_EL, listTheory.EL_APPEND_EQN]
+  >> ‘t' <= LENGTH M1’ by cheat (* wf invariant should cover this *)
+  >> fs[GSYM mem_get_is_loc, optionTheory.IS_SOME_EXISTS]
+  >> fs[mem_get_append]
   ,fs[]
   ,fs[]
   ,fs[]
@@ -315,12 +769,12 @@ Induct_on ‘clstep’
   >> fs[bir_programTheory.bir_state_t_accfupds]
   >> Q.LIST_EXISTS_TAC [‘v’,‘l’,‘v_addr’,‘v_data’,‘new_env’, ‘new_viewenv’]
   >> gvs[fulfil_atomic_ok_def, fulfil_update_env_def, fulfil_update_viewenv_def, listTheory.oEL_EQ_EL, listTheory.EL_APPEND_EQN]
+  >> ‘t <= LENGTH M1’ by cheat (* wf invariant *)
   >> rpt strip_tac
   >| [
-      Cases_on ‘s.bst_xclb’ >- fs[]
-      >> fs[] >> DISCH_TAC >> GEN_TAC >> rpt strip_tac
-      >> ‘t' < LENGTH M1 + 1’ by DECIDE_TAC
-      >> fs[]
+      fs[mem_is_cid_def] >> cheat (* proof obligation about mem_is_cide *)
+      ,
+      fs[mem_get_append]
       ,
       gvs[]
       >>
@@ -334,10 +788,21 @@ Induct_on ‘clstep’
   , (* amo *)
   HO_MATCH_MP_TAC (List.nth (CONJUNCTS clstep_rules,3))
   >> fs[bir_programTheory.bir_state_t_accfupds]
-  >> Q.LIST_EXISTS_TAC [‘v_addr’, ‘v_data’, ‘v_post’, ‘l’, ‘v_r’, ‘v_w’, ‘t_r’, ‘new_environ’]
+  >> Q.LIST_EXISTS_TAC [‘v_addr’, ‘v_data’, ‘l’, ‘v_r’, ‘v_w’, ‘t_r’, ‘new_environ’]
   >> gvs[fulfil_atomic_ok_def, fulfil_update_env_def, fulfil_update_viewenv_def, listTheory.oEL_EQ_EL, listTheory.EL_APPEND_EQN]
+  >> ‘t_w <= LENGTH M1’ by cheat (* wf invariant *)
   >> rpt strip_tac
   >| [drule mem_read_some >> strip_tac >> fs[mem_read_append]
+      ,
+      fs[mem_get_append]
+      ,
+      qpat_assum ‘!t''._’ (fn th => drule (Q.SPEC ‘t'’ th))
+      >> rpt strip_tac
+      >> ‘mem_is_loc M1 t' l’ by fs[]
+      >> fs[optionTheory.IS_SOME_EXISTS, GSYM mem_get_is_loc]
+      >> qexists_tac ‘x’
+      >> ‘t' <= LENGTH M1’ by decide_tac
+      >> fs[mem_get_append]
       ,
       gvs[]
       >>
@@ -371,8 +836,7 @@ Induct_on ‘clstep’
 >> rw[bir_exec_stmt_promise_commutes]
 ]
 QED
-  
-  
+
 Theorem certification_extension:
 !p cid M s s'' msg prom.
   is_certified p cid s'' M
@@ -397,44 +861,6 @@ Proof
   >> fs[cstep_seq_rtc_def]
   >> metis_tac[relationTheory.RTC_RULES]
 QED
-(*
-Theorem promise_parstep:
-!p cid s M2 msg T1.
-  FLOOKUP T1 cid = SOME (Core cid p s) /\
-     is_certified p cid (s with bst_prom updated_by (λpr. pr ⧺ [LENGTH M2 + 1])) (M2 ⧺ [msg]) /\ msg.cid = cid
-  ==>
-  parstep cid T1 M2
-  (FUPDATE T1 (cid, Core cid p
-                    (s with bst_prom updated_by (λpr. pr ⧺ [LENGTH M2 + 1]))))
-  (M2 ⧺ [msg])
-Proof
-    rpt strip_tac
-    >> ‘cstep p cid s M2 [LENGTH M2 + 1] (s with bst_prom updated_by (λpr. pr ⧺ [LENGTH M2 + 1])) (M2 ++ [msg])’ by fs[promise_cstep]
-    >> cheat
-QED
-
-Theorem promise_step_non_interference:
-! cid T1 M p p' s s' msg M1.
-         ~(cid = msg.cid) /\ parstep cid T1 M (T1 |+ (cid,Core cid p' s')) M
- /\ FLOOKUP (T1 |+ (cid,Core cid p' s')) msg.cid = SOME (Core msg.cid p s)
-==>
-parstep cid (T1 |+ (msg.cid, Core msg.cid p (s' with bst_prom updated_by (λpr. pr ⧺ [LENGTH M1 + 1])))) (M1 ++ [msg]) (T1 |+ (cid, Core cid p' s) |+ (msg.cid, Core msg.cid p (s with bst_prom updated_by (\pr. pr ++ [LENGTH M1 + 1])))) (M1 ++ [msg])
-Proof
-  fs[parstep_cases, parstep_rules] >> rpt strip_tac
->> cheat
-QED 
-*)
-val promise_subst = subst [“s:bir_state_t” |-> “(s with bst_prom updated_by (λpr. pr ⧺ [LENGTH M1 + 1]))”, “s':bir_state_t” |-> “(s' with bst_prom updated_by (λpr. pr ⧺ [LENGTH M1 + 1]))”];
-
-val case1 = “(s' :bir_state_t) =
-             (s :bir_state_t) with
-                              <|bst_v_rNew :=
-                                MAX s.bst_v_rNew
-                                    (if is_read (K2 :bir_memop_t) then (v :num) else (0 :num));
-                                bst_v_wNew :=
-                                MAX s.bst_v_wNew (if is_write K2 then v else (0 :num));
-                                bst_pc updated_by bir_pc_next|>”;
-
 
 Theorem nonpromising_extra_promise:
 !msg T1 p s' s M1.
@@ -454,32 +880,19 @@ Proof
   >> fs[cstep_cases, promises_do_not_disable_clsteps]
 QED
 
-Theorem programs_unchanged:
-!cid T1 T2 M1 M2.
-  parstep cid T1 M1 T2 M2 ==>
-     !p s p' s'.
-       FLOOKUP T1 cid = SOME (Core cid p s)
-       /\ FLOOKUP T2 cid = SOME (Core cid p' s')
-       ==> p = p'
-Proof
-   rpt strip_tac
->> fs[parstep_cases]
->> last_assum (fn th => fs [th,FLOOKUP_UPDATE])
-QED
-
 Theorem bir_promising_diamond_same_core:
   !T1 T2 T3 M1 M2 M3 cid.
   (nonpromise_step cid (T1,M1) (T2,M2) /\ promise_step cid (T2,M2) (T3,M3))
   ==>
   ?T1' T2' T3' M1' M2' M3'.
-       sim_rel (T1,M1) (T1',M1')
+       (T1,M1) = (T1',M1')
     /\ promise_step cid (T1',M1') (T2',M2')
     /\ nonpromise_step cid (T2',M2') (T3',M3')
-    /\ sim_rel (T3,M3) (T3',M3')
+    /\ (T3,M3) = (T3',M3')
 Proof
   REWRITE_TAC[bir_nonpromise_step_def, bir_promise_step_def]
 >> REPEAT STRIP_TAC
->> fs[sim_rel_eq]
+>> fs[]
 >> drule execute_inversion >> rw[]
 >> drule promise_inversion  >> rw[]
 >> fs[FLOOKUP_UPDATE] (* introduces p = p' and s = s'' *)
@@ -520,12 +933,14 @@ Proof
     [drule mem_read_some >> strip_tac >> fs[mem_read_append]
      ,fs[]
      , (* quantifier case *)
-     qpat_assum ‘!t''._’ (fn th => drule (Q.SPEC ‘t'’ th))
+     ‘t' <= LENGTH M’ by cheat (* wf invariant *)
+     >> qpat_assum ‘!t''._’ (fn th => drule (Q.SPEC ‘t'’ th))
      >> rpt strip_tac
      >> ‘t' ≤ MAX v_pre (s.bst_coh l)’ by fs[bir_state_t_accfupds]
-     >> ‘∃msg. oEL (t'-1) M = SOME msg ∧ msg.loc ≠ l’ by fs[]
-     >> Q.EXISTS_TAC ‘msg'’
-     >> fs[listTheory.oEL_EQ_EL, listTheory.EL_APPEND_EQN]
+     >> ‘~mem_is_loc M t' l’ by fs[]
+     >> fs[optionTheory.IS_SOME_EXISTS, GSYM mem_get_is_loc]
+     >> qpat_assum ‘!x._’ (fn th => assume_tac (Q.SPEC ‘x’ th))
+     >> fs[mem_get_append]
      ,fs[]
      ,fs[]
      ,fs[]
@@ -539,19 +954,29 @@ Proof
     >> fs[bir_programTheory.bir_state_t_accfupds]
     >> Q.LIST_EXISTS_TAC [‘v’,‘l’,‘v_addr’,‘v_data’,‘new_env’, ‘new_viewenv’]
     >> gvs[fulfil_atomic_ok_def, fulfil_update_env_def, fulfil_update_viewenv_def, listTheory.oEL_EQ_EL, listTheory.EL_APPEND_EQN]
-    >> rpt strip_tac
-    >> Cases_on ‘s.bst_xclb’ >- fs[]
-    >> fs[] >> DISCH_TAC >> GEN_TAC >> rpt strip_tac
-    >> ‘t' < LENGTH M + 1’ by DECIDE_TAC
-    >> fs[]
+    >> rpt strip_tac >- cheat (* mem_is_cid *)
+    >> ‘t <= LENGTH M’ by cheat (* wf invariant *)
+    >> fs[mem_get_append]
     ,(* amo *)
     HO_MATCH_MP_TAC (List.nth (CONJUNCTS clstep_rules,3))
     >> fs[bir_programTheory.bir_state_t_accfupds]
-    >> Q.LIST_EXISTS_TAC [‘v_addr’, ‘v_data’, ‘v_post’, ‘l’, ‘v_r’, ‘v_w’, ‘t_r’, ‘new_environ’]
+    >> Q.LIST_EXISTS_TAC [‘v_addr’, ‘v_data’, ‘l’, ‘v_r’, ‘v_w’, ‘t_r’, ‘new_environ’]
+    >> ‘t_w <= LENGTH M’ by cheat (* wf invariant *)
     >> gvs[fulfil_atomic_ok_def, fulfil_update_env_def, fulfil_update_viewenv_def, listTheory.oEL_EQ_EL, listTheory.EL_APPEND_EQN]
-    >> drule mem_read_some
-    >> strip_tac
-    >> fs[mem_read_append]
+    >> rpt strip_tac
+    >| [
+        drule mem_read_some >> strip_tac >> fs[mem_read_append]
+        ,
+        fs[mem_get_append]
+        ,
+        qpat_assum ‘!t'._’ (fn th => drule (Q.SPEC ‘t'’ th))
+        >> strip_tac
+        >> ‘mem_is_loc M t' l’ by fs[]
+        >> fs[optionTheory.IS_SOME_EXISTS, GSYM mem_get_is_loc]
+        >> qexists_tac ‘x’
+        >> ‘t' <= LENGTH M’ by decide_tac
+        >> fs[mem_get_append]
+      ]
     ,
   HO_MATCH_MP_TAC (List.nth (CONJUNCTS clstep_rules,4))
   >> fs[bir_programTheory.bir_state_t_accfupds]
@@ -571,80 +996,21 @@ Proof
   ]
 QED
 
-Triviality mem_read_take:
-  !m n l M v.
-  m <= n /\ n <= LENGTH M ==> mem_read (TAKE n M) l m = mem_read M l m
-Proof
-  Induct_on ‘m’
-  >> fs[mem_read_def, mem_read_aux_def]
-  >> rpt strip_tac
-  >> ‘m <= n’ by decide_tac
-  >> ‘m <= LENGTH M’ by decide_tac
-  >> ‘m <= LENGTH (TAKE n M)’ by fs[]
-  >> fs[listTheory.oEL_THM]
-  >> fs[mem_read_def, mem_read_aux_def]
-  >> fs[listTheory.EL_TAKE]
-QED
+(* Latest version of the NI-like lemma
+if the step is a load
 
-Definition is_read_def:
-  is_read p s =
-  ?var a_e opt_cast xcl acq rel.
-    bir_get_stmt p s.bst_pc =
-    BirStmt_Read var a_e opt_cast xcl acq rel
-End
-
-Theorem gen_promises_do_not_disable_clsteps_other_core:
-  !p cid M prom s s' msg idx.
-    ~(cid = msg.cid)
-    /\ clstep p cid s M prom s'
-    /\ ~(is_read p s) /\ 0 < idx /\ idx < LENGTH M
-    ==>
-    ?prom'.clstep p cid s (LINSERT msg idx M) prom' s'
+Theorem cstep_seq_views_lower_bound:
+  cstep_seq p cid (s,M) (s,M')
+  /\ M' = M
+  /\ is_read_stmt p s l t v_pre
+  /\ t <> 0
+  /\ t <= (MAX v_pre s.bst_coh l)
+==>
+  t = v_pre \/ t = s.bst_coh l
 Proof
-  fs[LINSERT_def, is_read_def]
-  >> Induct_on ‘clstep’
-  >> rpt strip_tac >- fs[] >> WEAKEN_TAC is_forall
-  >| [ 
-    (* xclfail *)
-    qexists_tac ‘[]’
-    >> HO_MATCH_MP_TAC (List.nth (CONJUNCTS clstep_rules,1))
-    >> Q.LIST_EXISTS_TAC [‘a_e’, ‘v_e’, ‘acq’, ‘rel’, ‘new_env’, ‘new_viewenv’]
-    >> fs[xclfail_update_env_def, xclfail_update_viewenv_def]
-    ,(* fulfil *)
-    Cases_on ‘idx > t’
-    >| [
-        qexists_tac ‘[t]’
-        >> HO_MATCH_MP_TAC (List.nth (CONJUNCTS clstep_rules,2))
-        >> fs[bir_programTheory.bir_state_t_accfupds]
-        >> Q.LIST_EXISTS_TAC [‘v’,‘l’,‘v_addr’,‘v_data’,‘new_env’, ‘new_viewenv’]
-        >> gvs[listTheory.oEL_EQ_EL, listTheory.EL_APPEND_EQN]
-        >> fs[fulfil_atomic_ok_def]
-(*        >> gvs[fulfil_atomic_ok_def, fulfil_update_env_def, fulfil_update_viewenv_def, listTheory.oEL_EQ_EL, listTheory.EL_APPEND_EQN] *)
-        >> rpt strip_tac
-        >- (Cases_on ‘s.bst_xclb’ >- fs[]
-            >> fs[]
-            >> rpt strip_tac)
-      ]
-        , (* amo *)
   cheat
-  ,
-  HO_MATCH_MP_TAC (List.nth (CONJUNCTS clstep_rules,3))
-  >> fs[bir_programTheory.bir_state_t_accfupds]
-  ,
-  HO_MATCH_MP_TAC (List.nth (CONJUNCTS clstep_rules,4))
-  >> fs[bir_programTheory.bir_state_t_accfupds]
-  >> Q.LIST_EXISTS_TAC [‘v’, ‘oo’, ‘s2’, ‘v_addr’]
-  >> rw[bir_exec_stmt_promise_commutes]
-  ,
-  HO_MATCH_MP_TAC (List.nth (CONJUNCTS clstep_rules,5))
-  >> fs[bir_programTheory.bir_state_t_accfupds]
-  >> Q.LIST_EXISTS_TAC [‘v’, ‘v_val’, ‘new_env’]
-  >> fs[]
-  ,
-  HO_MATCH_MP_TAC (List.nth (CONJUNCTS clstep_rules,6))
-  >> rpt HINT_EXISTS_TAC >> fs[]
-  ]
 QED
+ *)
 
 Theorem promises_other_core_commute_alt:
   !p msg1 msg2 s M M'.
@@ -670,6 +1036,7 @@ Proof
   >> fs[cstep_cases]
 QED
 
+(* This approach does not seem to work *)
 Theorem clstep_fulfil_other_core:
 !p msg' msg s M s'.
 (~(msg.cid = msg'.cid)
@@ -688,33 +1055,6 @@ Proof
       >> cheat
   ,
   cheat]
-QED
-
-Definition LINSERT_def:
-  LINSERT x t xs = TAKE (t-1) xs ++ x :: DROP (t-1) xs
-End
-
-Theorem gen_promise_does_not_disable_cstep_seq:
-!cid msg p s M s' M' t.
-   (~(cid = msg.cid)
-    /\ cstep_seq p cid (s,M) (s',M'))
- ==>
-   cstep_seq p cid (s,LINSERT msg t M) (s',LINSERT msg t M')
-Proof
-  rpt strip_tac
-  >> gs[cstep_seq_cases]
-  >| [
-      >> qexists_tac ‘prom’
-      >> qexists_tac ‘new_env’
-      >> qexists_tac ‘new_viewenv’
-
-Induct_on ‘R1’ using listTheory.SNOC_INDUCT
-      >- (strip_tac
-          >> drule_all promises_do_not_disable_clsteps_other_core
-          >> rw[]
-          >> Q.EXISTS_TAC ‘prom’ >> fs[])
-      >> rpt strip_tac
-     ]
 QED
 
 Theorem promise_list_does_not_disable_cstep_seq:
@@ -751,6 +1091,8 @@ Proof
      ]
 QED
 
+(* Some minor lemmas about cstep_seq *)
+
 Theorem cstep_seq_memory_only_grows:
   !p cid x y.
     cstep_seq p cid x y
@@ -773,40 +1115,9 @@ Proof
   >> rpt strip_tac >- (Q.EXISTS_TAC ‘[]’ >> fs[])
   >> fs[cstep_seq_cases, cstep_cases]
 QED
-  
-Theorem cstep_seq_rtc_monotonicity:
-  !cid p M2 x y.
-    (!m. MEM m M2 ==> ~(cid = m.cid))
-    ==> cstep_seq_rtc p cid x y
-    ==> cstep_seq_rtc p cid
-                  (FST x, SND x ++ M2)
-                  (FST y, SND x ++ M2 ++ (DROP (LENGTH (SND x)) (SND y)))
-Proof
-  cheat
-QED
 
-(*  
-Theorem promises_do_not_disable_cstep_seq_rtc:
-  !cid msg p x y MSUFF.
-    (~(cid = msg.cid)
-     /\ cstep_seq_rtc p cid x y
-     /\ SND y = SND x ++ MSUFF)
-    ==>
-    cstep_seq_rtc p cid (FST x,SND x++[msg]) (FST y,SND x ++ [msg] ++ MSUFF)
-Proof
-  gen_tac >> gen_tac >> gen_tac
-  >> fs[cstep_seq_rtc_def]
-  >> Induct_on ‘(cstep_seq p cid)꙳’ using relationTheory.RTC_STRONG_INDUCT_RIGHT1 
-  >> rpt strip_tac >- (fs[])
-  >> fs[]
-  >> PairCases_on ‘x’
-  >> PairCases_on ‘y'’
-  >> PairCases_on ‘y’
-  >> fs[]
-  >> drule cstep_seq_memory_only_grows >> rw[]
-  >> drule_all promises_do_not_disable_cstep_seq >> rw[]
-QED
-*)
+(*
+Failed proof attempt:
 
 Theorem certification_extension_other_core:
 !p p' cid s s' s'' M prom msg.
@@ -830,7 +1141,10 @@ Proof
   >> fs[cstep_seq_rtc_def]
   >> metis_tac[relationTheory.RTC_RULES]
 QED
+*)
 
+(* The following lemma is needed in the
+bir_promising_diamond_diff_core proof *)
 Theorem certification_extension_other_core:
   !p p' cid s s' s'' M prom msg.
     ~(cid = msg.cid)
@@ -850,14 +1164,13 @@ Theorem bir_promising_diamond_diff_core:
     /\ promise_step cid2 (T2,M2) (T3,M3))
     ==>
     ?T1' T2' T3' M1' M2' M3'.
-      sim_rel (T1,M1) (T1',M1')
+      (T1,M1) = (T1',M1')
       /\ promise_step cid2 (T1',M1') (T2',M2')
       /\ nonpromise_step cid1 (T2',M2') (T3',M3')
-      /\ sim_rel (T3,M3) (T3',M3')
+      /\ (T3,M3) = (T3',M3')
 Proof
-  REWRITE_TAC[bir_nonpromise_step_def, bir_promise_step_def]
-  >> REPEAT STRIP_TAC
-  >> fs[sim_rel_eq]
+  fs[bir_nonpromise_step_def, bir_promise_step_def]
+  >> rpt strip_tac
   >> drule execute_inversion >> rw[]
   >> drule promise_inversion  >> rw[]
   >> fs[FLOOKUP_UPDATE]
